Power_Products_PM.thy
@@ -1,0 +1,435 @@
+theory Power_Products_PM
+  imports "HOL-Library.Function_Algebras" Number_Classes
+begin
+
+section \<open>Power-Products Represented by Polynomial Mappings\<close>
+
+subsection \<open>Natural and Integer-Valued Polynomial Mappings\<close>
+
+lift_definition of_nat_pm :: "('a \<Rightarrow>\<^sub>0 nat) \<Rightarrow> ('a \<Rightarrow>\<^sub>0 'b::semiring_1)" is of_nat_fun
+proof -
+  fix f::"'a \<Rightarrow> nat"
+  have "{x. of_nat_fun f x \<noteq> 0} \<subseteq> {x. f x \<noteq> 0}"
+  proof (rule, simp add: of_nat_fun_def)
+    fix x
+    assume "of_nat (f x) \<noteq> 0"
+    have "f x \<noteq> 0"
+    proof
+      assume "f x = 0"
+      hence "of_nat (f x) = 0" by simp
+      with \<open>of_nat (f x) \<noteq> 0\<close> show False ..
+    qed
+    thus "0 < f x" by simp
+  qed
+  moreover assume "finite {x. f x \<noteq> 0}"
+  ultimately show "finite {x. of_nat_fun f x \<noteq> 0}" by (rule finite_subset)
+qed
+
+lift_definition of_int_pm :: "('a \<Rightarrow>\<^sub>0 int) \<Rightarrow> ('a \<Rightarrow>\<^sub>0 'b::ring_1)" is of_int_fun
+proof -
+  fix f::"'a \<Rightarrow> int"
+  have "{x. of_int_fun f x \<noteq> 0} \<subseteq> {x. f x \<noteq> 0}"
+  proof (rule, simp add: of_int_fun_def, rule)
+    fix x
+    assume "of_int (f x) \<noteq> 0"
+    assume "f x = 0"
+    hence "of_int (f x) = 0" by simp
+    with \<open>of_int (f x) \<noteq> 0\<close> show False ..
+  qed
+  moreover assume "finite {x. f x \<noteq> 0}"
+  ultimately show "finite {x. of_int_fun f x \<noteq> 0}" by (rule finite_subset)
+qed
+
+lift_definition of_rat_pm :: "('a \<Rightarrow>\<^sub>0 rat) \<Rightarrow> ('a \<Rightarrow>\<^sub>0 'b::field_char_0)" is of_rat_fun
+proof -
+  fix f::"'a \<Rightarrow> rat"
+  have "{x. of_rat_fun f x \<noteq> 0} \<subseteq> {x. f x \<noteq> 0}" by (rule, simp add: of_rat_fun_def)
+  moreover assume "finite {x. f x \<noteq> 0}"
+  ultimately show "finite {x. of_rat_fun f x \<noteq> 0}" by (rule finite_subset)
+qed
+
+lemma lookup_of_nat_pm: "lookup (of_nat_pm t) x = of_nat (lookup t x)"
+  by (simp add: of_nat_fun_def of_nat_pm.rep_eq)
+
+lemma lookup_of_int_pm: "lookup (of_int_pm t) x = of_int (lookup t x)"
+  by (simp add: of_int_fun_def of_int_pm.rep_eq)
+
+lemma lookup_of_rat_pm: "lookup (of_rat_pm t) x = of_rat (lookup t x)"
+  by (simp add: of_rat_fun_def of_rat_pm.rep_eq)
+
+lift_definition to_nat_pm :: "('a \<Rightarrow>\<^sub>0 'b::floor_ceiling) \<Rightarrow> ('a \<Rightarrow>\<^sub>0 nat)" is to_nat_fun
+proof -
+  fix f::"'a \<Rightarrow> 'b"
+  have "{x. to_nat_fun f x \<noteq> 0} \<subseteq> {x. f x \<noteq> 0}"
+  proof (rule, simp add: to_nat_fun_def, rule)
+    fix x
+    assume "0 < to_nat (f x)"
+    hence "to_nat (f x) \<noteq> 0" by simp
+    assume "f x = 0"
+    hence "to_nat (f x) = 0" by (simp add: to_nat_def)
+    with \<open>to_nat (f x) \<noteq> 0\<close> show False ..
+  qed
+  moreover assume "finite {x. f x \<noteq> 0}"
+  ultimately show "finite {x. to_nat_fun f x \<noteq> 0}" by (rule finite_subset)
+qed
+
+lift_definition to_int_pm :: "('a \<Rightarrow>\<^sub>0 'b::floor_ceiling) \<Rightarrow> ('a \<Rightarrow>\<^sub>0 int)" is to_int_fun
+proof -
+  fix f::"'a \<Rightarrow> 'b"
+  have "{x. to_int_fun f x \<noteq> 0} \<subseteq> {x. f x \<noteq> 0}" by (rule, simp add: to_int_fun_def, rule, simp)
+  moreover assume "finite {x. f x \<noteq> 0}"
+  ultimately show "finite {x. to_int_fun f x \<noteq> 0}" by (rule finite_subset)
+qed
+
+lemma lookup_to_nat_pm: "lookup (to_nat_pm t) x = to_nat (lookup t x)"
+  by (simp add: to_nat_fun_def to_nat_pm.rep_eq)
+
+lemma lookup_to_int_pm: "lookup (to_int_pm t) x = floor (lookup t x)"
+  by (simp add: to_int_fun_def to_int_pm.rep_eq)
+
+definition is_nat_pm where "is_nat_pm t = is_nat_fun (lookup t)"
+definition is_int_pm where "is_int_pm t = is_int_fun (lookup t)"
+
+lemma is_nat_pmI:
+  assumes "\<And>x. x \<in> keys t \<Longrightarrow> is_nat (lookup t x)"
+  shows "is_nat_pm t"
+  unfolding is_nat_pm_def is_nat_fun_def
+proof
+  fix x
+  show "is_nat (lookup t x)"
+  proof (cases "x \<in> keys t")
+    case True
+    thus ?thesis by (rule assms)
+  next
+    case False
+    hence "lookup t x = 0" by simp
+    thus ?thesis by (simp add: zero_is_nat)
+  qed
+qed
+
+lemma is_nat_pmD:
+  assumes "is_nat_pm t"
+  shows "is_nat (lookup t x)"
+  using assms unfolding is_nat_pm_def is_nat_fun_def ..
+
+lemma is_int_pmI:
+  assumes "\<And>x. x \<in> keys t \<Longrightarrow> is_int (lookup t x)"
+  shows "is_int_pm t"
+  unfolding is_int_pm_def is_int_fun_def
+proof
+  fix x
+  show "is_int (lookup t x)"
+  proof (cases "x \<in> keys t")
+    case True
+    thus ?thesis by (rule assms)
+  next
+    case False
+    hence "lookup t x = 0" by simp
+    thus ?thesis by (simp add: is_int_def)
+  qed
+qed
+
+lemma is_int_pmD:
+  assumes "is_int_pm t"
+  shows "is_int (lookup t x)"
+  using assms unfolding is_int_pm_def is_int_fun_def ..
+
+lemma nat_pm_is_int_pm:
+  assumes "is_nat_pm t"
+  shows "is_int_pm t"
+proof (rule is_int_pmI)
+  fix x
+  from assms have "is_nat (lookup t x)" by (rule is_nat_pmD)
+  thus "is_int (lookup t x)" by (rule nat_is_int)
+qed
+
+lemma int_pm_is_nat_pm:
+  assumes "is_int_pm t" and "\<And>x. x \<in> keys t \<Longrightarrow> 0 \<le> lookup t x"
+  shows "is_nat_pm t"
+  unfolding is_nat_pm_def is_nat_fun_def
+proof
+  fix x
+  show "is_nat (lookup t x)"
+  proof (cases "x \<in> keys t")
+    case True
+    from assms(1) have "is_int (lookup t x)" unfolding is_int_pm_def is_int_fun_def ..
+    moreover from True have "0 \<le> lookup t x" by (rule assms(2))
+    ultimately show ?thesis by (rule int_is_nat)
+  next
+    case False
+    hence "lookup t x = 0" by simp
+    thus ?thesis by (simp add: zero_is_nat)
+  qed
+qed
+
+lemma of_nat_pm_is_nat_pm: "is_nat_pm (of_nat_pm f)"
+  by (simp add: is_nat_pm_def is_nat_fun_def lookup_of_nat_pm of_nat_is_nat)
+
+lemma of_int_pm_is_int_pm: "is_int_pm (of_int_pm f)"
+  by (simp add: is_int_pm_def is_int_fun_def lookup_of_int_pm of_int_is_int)
+
+lemma lcs_of_nat_pm:
+  assumes "\<And>m n::nat. of_nat m \<le> ((of_nat n)::'b::{semiring_1, add_linorder}) \<longleftrightarrow> m \<le> n"
+  shows "lcs (of_nat_pm a) (of_nat_pm b) = ((of_nat_pm (lcs a b))::'a \<Rightarrow>\<^sub>0 'b)"
+  by (transfer, auto simp add: of_nat_fun_def max_of_nat[OF assms])
+
+lemma lookup_gcs_fun_stronger: "lookup (gcs s (t::'a \<Rightarrow>\<^sub>0 ('b::add_linorder))) = gcs (lookup s) (lookup t)"
+proof
+  fix x
+  show "lookup (gcs s t) x = gcs (lookup s) (lookup t) x"
+    by (simp add: gcs_def lookup_minus lookup_add lookup_lcs_fun)
+qed
+
+lemma gcs_of_nat_pm:
+  assumes "\<And>m n::nat. of_nat m \<le> ((of_nat n)::'b::{semiring_1, add_linorder}) \<longleftrightarrow> m \<le> n"
+  shows "gcs (of_nat_pm a) (of_nat_pm b) = ((of_nat_pm (gcs a b))::'a \<Rightarrow>\<^sub>0 'b)"
+  by (rule poly_mapping_eqI, simp add: lookup_gcs_fun_stronger of_nat_pm.rep_eq gcs_fun of_nat_fun_def,
+      auto simp add: min_of_nat[OF assms])
+
+lemmas lcs_of_nat_pm_linordered_semidom = lcs_of_nat_pm[OF Nat.linordered_semidom_class.of_nat_le_iff]
+lemmas gcs_of_nat_pm_linordered_semidom = gcs_of_nat_pm[OF Nat.linordered_semidom_class.of_nat_le_iff]
+  
+lemma lcs_is_nat_pm:
+  assumes "is_nat_pm f" and "is_nat_pm g"
+  shows "is_nat_pm (lcs f g)"
+  using assms unfolding is_nat_pm_def lookup_lcs_fun unfolding lcs_fun_def is_nat_fun_def
+  using max_is_nat by auto
+    
+lemma lcs_is_nat_pm':
+  assumes "is_nat_pm f" and "is_int_pm g"
+  shows "is_nat_pm (lcs f g)"
+  using assms unfolding is_nat_pm_def is_int_pm_def lookup_lcs_fun
+  unfolding lcs_fun_def is_nat_fun_def is_int_fun_def using max_is_nat' by auto
+
+lemma lcs_is_int_pm:
+  assumes "is_int_pm f" and "is_int_pm g"
+  shows "is_int_pm (lcs f g)"
+  using assms unfolding is_int_pm_def lookup_lcs_fun unfolding lcs_fun_def is_int_fun_def
+  using max_is_int by auto
+
+lemma gcs_is_nat_pm:
+  assumes "is_nat_pm f" and "is_nat_pm g"
+  shows "is_nat_pm (gcs f g)"
+  using assms unfolding is_nat_pm_def lookup_gcs_fun_stronger unfolding gcs_fun is_nat_fun_def
+  using min_is_nat by auto
+
+lemma gcs_is_int_pm:
+  assumes "is_int_pm f" and "is_int_pm g"
+  shows "is_int_pm (gcs f g)"
+  using assms unfolding is_int_pm_def lookup_gcs_fun_stronger unfolding gcs_fun is_int_fun_def
+  using min_is_int by auto
+  
+lemma zero_is_nat_pm [simp]: "is_nat_pm 0"
+  unfolding is_nat_pm_def lookup_zero is_nat_fun_def using zero_is_nat by simp
+
+lemma of_nat_pm_zero [simp]: "of_nat_pm 0 = 0"
+  by (rule poly_mapping_eqI, simp add: lookup_of_nat_pm)
+
+lemma of_int_pm_zero [simp]: "of_int_pm 0 = 0"
+  by (rule poly_mapping_eqI, simp add: lookup_of_int_pm)
+  
+lemma plus_is_nat_pm:
+  assumes "is_nat_pm f" and "is_nat_pm g"
+  shows "is_nat_pm (f + g)"
+  using assms unfolding is_nat_pm_def plus_poly_mapping.rep_eq unfolding plus_fun_def is_nat_fun_def
+  using plus_is_nat by auto
+
+lemma diff_is_nat_pm:
+  assumes "is_int_pm f" and "is_int_pm g"
+  shows "is_nat_pm (f - g) \<longleftrightarrow> lookup g \<le> lookup f"
+proof -
+  from assms have a2: "is_int (lookup f x)" and a3: "is_int (lookup g x)" for x
+    by (simp_all add: is_int_pm_def is_int_fun_def)
+  show ?thesis
+  proof
+    assume "is_nat_pm (f - g)"
+    hence a1: "is_nat (lookup (f - g) x)" for x unfolding is_nat_pm_def is_nat_fun_def ..
+    
+    show "lookup g \<le> lookup f" unfolding le_fun_def
+    proof
+      fix x
+      from a1 have "is_nat ((lookup f x) - (lookup g x))" by (simp only: lookup_minus)
+      thus "lookup g x \<le> lookup f x" unfolding diff_is_nat[OF a2 a3] .
+    qed
+  next
+    assume "lookup g \<le> lookup f"
+    show "is_nat_pm (f - g)" unfolding is_nat_pm_def is_nat_fun_def
+    proof
+      fix x
+      from \<open>lookup g \<le> lookup f\<close> have "lookup g x \<le> lookup f x" unfolding le_fun_def ..
+      hence "is_nat ((lookup f x) - (lookup g x))" unfolding diff_is_nat[OF a2 a3] .
+      thus "is_nat (lookup (f - g) x)" by (simp only: lookup_minus)
+    qed
+  qed
+qed
+
+lemma plus_is_int_pm:
+  assumes "is_int_pm f" and "is_int_pm g"
+  shows "is_int_pm (f + g)"
+  using assms unfolding is_int_pm_def plus_poly_mapping.rep_eq unfolding plus_fun_def is_int_fun_def
+  using plus_is_int by auto
+
+lemma diff_is_int_pm:
+  assumes "is_int_pm f" and "is_int_pm g"
+  shows "is_int_pm (f - g)"
+  using assms unfolding is_int_pm_def lookup_minus is_int_fun_def using diff_is_int by auto
+
+lemma minus_is_int_pm:
+  assumes "is_int_pm f"
+  shows "is_int_pm (- f)"
+  using assms unfolding is_int_pm_def is_int_fun_def using minus_is_int by auto
+
+lemma of_nat_pm_plus: "of_nat_pm (f + g) = of_nat_pm f + of_nat_pm g"
+  by (rule poly_mapping_eqI, simp add: lookup_of_nat_pm lookup_add)
+
+lemma of_int_pm_plus: "of_int_pm (f + g) = of_int_pm f + of_int_pm g"
+  by (rule poly_mapping_eqI, simp add: lookup_of_int_pm lookup_add)
+
+subsubsection \<open>Composition\<close>
+
+lemma to_int_pm_comp_of_int_pm [simp]: "to_int_pm (of_int_pm t) = t"
+  by (rule poly_mapping_eqI, simp add: lookup_to_int_pm lookup_of_int_pm)
+
+lemma to_nat_pm_comp_of_nat_pm [simp]: "to_nat_pm (of_nat_pm t) = t"
+  by (rule poly_mapping_eqI, simp add: lookup_to_nat_pm lookup_of_nat_pm to_nat_def)
+
+lemma to_nat_pm_comp_of_int_pm [simp]: "lookup (to_nat_pm (of_int_pm t)) = nat \<circ> (lookup t)"
+  by (simp add: to_nat_pm.rep_eq of_int_pm.rep_eq to_nat_fun_comp_of_int_fun)
+
+lemma of_nat_pm_comp_to_nat_pm:
+  assumes "is_nat_pm t"
+  shows "of_nat_pm (to_nat_pm t) = t"
+  using assms
+  by (simp add: is_nat_pm_def poly_mapping_eq_iff of_nat_pm.rep_eq to_nat_pm.rep_eq,
+      intro of_nat_fun_comp_to_nat_fun)
+
+lemma of_nat_pm_comp_to_nat_pm_eq_to_int_pm:
+  assumes "is_nat_pm (t::'a \<Rightarrow>\<^sub>0 'b::floor_ceiling)"
+  shows "of_nat_pm (to_nat_pm t) = to_int_pm t"
+  using assms
+  by (simp add: is_nat_pm_def poly_mapping_eq_iff of_nat_pm.rep_eq to_nat_pm.rep_eq to_int_pm.rep_eq,
+      intro of_nat_fun_comp_to_nat_fun_eq_to_int_fun)
+
+lemma of_int_pm_comp_to_int_pm:
+  assumes "is_int_pm t"
+  shows "of_int_pm (to_int_pm t) = t"
+  using assms
+  by (simp add: is_int_pm_def poly_mapping_eq_iff of_int_pm.rep_eq to_int_pm.rep_eq,
+      intro of_int_fun_comp_to_int_fun)
+
+lemma of_int_pm_comp_of_nat_pm [simp]: "of_int_pm (of_nat_pm t) = of_nat_pm t"
+  by (simp add: poly_mapping_eq_iff of_int_pm.rep_eq of_nat_pm.rep_eq, fact of_int_fun_comp_of_nat_fun)
+
+subsection \<open>Order relation on polynomial mappings\<close>
+
+definition le_pm :: "('a \<Rightarrow>\<^sub>0 'b) \<Rightarrow> ('a \<Rightarrow>\<^sub>0 'b::{ord,zero}) \<Rightarrow> bool" (infixl "\<unlhd>" 50)
+  where "le_pm s t \<longleftrightarrow> (lookup s \<le> lookup t)"
+
+lemma le_pmI:
+  assumes "\<And>x. lookup s x \<le> lookup t x"
+  shows "s \<unlhd> t"
+  unfolding le_pm_def le_fun_def using assms ..
+
+lemma le_pmD:
+  assumes "s \<unlhd> t"
+  shows "lookup s x \<le> lookup t x"
+  using assms unfolding le_pm_def le_fun_def ..
+
+lemma adds_pmI:
+  assumes "s \<unlhd> t"
+  shows "s adds (t::'a \<Rightarrow>\<^sub>0 'b::add_linorder)"
+  using assms by (simp add: le_pm_def, intro adds_poly_mappingI)
+
+lemma adds_pm: "s adds t \<longleftrightarrow> s \<unlhd> t"
+  for s t::"'a \<Rightarrow>\<^sub>0 'b::add_linorder_min"
+  by (simp add: adds_poly_mapping le_pm_def)
+
+lemma le_of_nat_pm: "of_nat_pm s \<unlhd> ((of_nat_pm t)::'a \<Rightarrow>\<^sub>0 ('b::linordered_semidom)) \<longleftrightarrow> s \<unlhd> t"
+  by (simp add: le_pm_def of_nat_pm.rep_eq leq_of_nat_fun)
+
+lemma le_of_int_pm: "of_int_pm s \<unlhd> ((of_int_pm t)::'a \<Rightarrow>\<^sub>0 ('b::linordered_idom)) \<longleftrightarrow> s \<unlhd> t"
+  by (simp add: le_pm_def of_int_pm.rep_eq leq_of_int_fun)
+
+lemma le_to_nat_pm:
+  assumes "s \<unlhd> t"
+  shows "to_nat_pm s \<unlhd> to_nat_pm t"
+  using assms by (simp add: le_pm_def to_nat_pm.rep_eq leq_to_nat_fun)
+
+lemma le_to_int_pm:
+  assumes "s \<unlhd> t"
+  shows "to_int_pm s \<unlhd> to_int_pm t"
+  using assms by (simp add: le_pm_def to_int_pm.rep_eq leq_to_int_fun)
+
+subsection \<open>Module-structure of polynomial mappings\<close>
+
+lift_definition scalar_mult_pm :: "'b \<Rightarrow> ('a \<Rightarrow>\<^sub>0 'b) \<Rightarrow> ('a \<Rightarrow>\<^sub>0 'b::mult_zero)" (infixl "\<cdot>" 70)
+  is "\<lambda>k f x. k * (f x)"
+  by (rule finite_mult_not_eq_zero_leftI)
+
+text \<open>If @{term t} is interpreted as a power-product, @{term "k \<cdot> t"} corresponds to exponentiation.\<close>
+
+lemma lookup_scalar_mult_pm [simp]: "lookup (k \<cdot> t) x = k * lookup t x"
+  by (transfer, simp)
+
+lemma scalar_zero_left [simp]: "(0::'b::mult_zero) \<cdot> t = 0"
+  by (rule poly_mapping_eqI, simp)
+
+lemma scalar_zero_right [simp]: "(k::'b::mult_zero) \<cdot> 0 = 0"
+  by (rule poly_mapping_eqI, simp)
+
+lemma scalar_one_left [simp]: "(1::'b::{mult_zero,monoid_mult}) \<cdot> t = t"
+  by (rule poly_mapping_eqI, simp)
+
+lemma scalar_distrib_left: "(k::'b::semiring_0) \<cdot> (s + t) = k \<cdot> s + k \<cdot> t"
+  by (rule poly_mapping_eqI, simp add: lookup_add distrib_left)
+
+lemma scalar_distrib_right: "(k + (l::'b::semiring_0)) \<cdot> t = k \<cdot> t + l \<cdot> t"
+  by (rule poly_mapping_eqI, simp add: lookup_add distrib_right)
+
+lemma scalar_Suc: "(Suc k) \<cdot> t = k \<cdot> t + t"
+  by (rule poly_mapping_eqI, simp add: lookup_add distrib_right)
+
+lemma scalar_uminus_left: "(-k::'b::ring) \<cdot> p = - (k \<cdot> p)"
+  by (rule poly_mapping_eqI, auto)
+
+lemma scalar_uminus_right: "(k::'b::ring) \<cdot> (-p) = - (k \<cdot> p)"
+  by (rule poly_mapping_eqI, auto)
+
+lemma scalar_minus_distrib_left: "(k::'b::comm_semiring_1_cancel) \<cdot> (p - q) = k \<cdot> p - k \<cdot> q"
+  by (rule poly_mapping_eqI, auto simp add: lookup_minus right_diff_distrib')
+
+lemma scalar_minus_distrib_right: "(k - (l::'b::comm_semiring_1_cancel)) \<cdot> f = k \<cdot> f - l \<cdot> f"
+  by (rule poly_mapping_eqI, auto simp add: lookup_minus left_diff_distrib')
+
+lemma scalar_is_nat_pm:
+  assumes "is_nat c" and "is_nat_pm t"
+  shows "is_nat_pm (c \<cdot> t)"
+  using assms unfolding is_nat_pm_def is_nat_fun_def using times_is_nat by auto
+
+lemma scalar_is_int_fun:
+  assumes "is_int c" and "is_int_pm t"
+  shows "is_int_pm (c \<cdot> t)"
+  using assms unfolding is_int_pm_def is_int_fun_def using times_is_int by auto
+
+subsection \<open>Locale @{term pm_powerprod}\<close>
+
+definition poly_deg :: "(('n \<Rightarrow>\<^sub>0 'a::add_linorder) \<Rightarrow>\<^sub>0 'b::zero) \<Rightarrow> 'a" where
+  "poly_deg p = (if keys p = {} then 0 else Max (deg_pm ` keys p))"
+
+definition maxdeg :: "(('n \<Rightarrow>\<^sub>0 'a::add_linorder) \<Rightarrow>\<^sub>0 'b::zero) set \<Rightarrow> 'a" where
+  "maxdeg A = Max (poly_deg ` A)"
+  
+definition mindeg :: "(('n \<Rightarrow>\<^sub>0 'a::add_linorder) \<Rightarrow>\<^sub>0 'b::zero) set \<Rightarrow> 'a" where
+  "mindeg A = Min (poly_deg ` A)"
+
+locale pm_powerprod =
+  ordered_powerprod ord ord_strict
+  for ord::"('n::countable \<Rightarrow>\<^sub>0 nat) \<Rightarrow> ('n \<Rightarrow>\<^sub>0 nat) \<Rightarrow> bool" (infixl "\<preceq>" 50)
+  and ord_strict (infixl "\<prec>" 50)
+begin
+
+sublocale gd_powerprod ..
+
+end
+
+end (* theory *)
